pulse/share/pulse/examples/dice/dpe/DPE.Trace.fsti
@@ -23,192 +23,158 @@ open EngineCore
 
 module SZ = FStar.SizeT
 module U8 = FStar.UInt8
+module U32 = FStar.UInt32
 
 let bytes = Seq.seq U8.t
 let lbytes (n:nat) = b:bytes { Seq.length b == n }
 let uds_t = lbytes (SZ.v uds_len)
 
-val ctxt_hndl_t : Type0
+type ctxt_hndl_t : Type0 = U32.t
 
 noeq
-type state_t : Type u#1 =
-  | SessionStart:
-      history:option state_t ->
-      state_t
+type g_session_state : Type u#1 =
+  | G_UnInitialized : g_session_state
+  | G_SessionStart : g_session_state
+  | G_Available : context_repr_t -> g_session_state
+  | G_InUse : g_session_state -> g_session_state
+  | G_SessionClosed : g_session_state -> g_session_state
+  | G_SessionError : g_session_state -> g_session_state
 
-  | EngineInitialized:
-      hndl:ctxt_hndl_t ->
-      uds:bytes ->
-      state_t
+let rec next (s0 s1:g_session_state) : prop =
+  match s0, s1 with
+  | G_UnInitialized, G_SessionStart -> True
 
-  | L0:
-      hndl:ctxt_hndl_t ->
-      uds:bytes ->
-      cdi:bytes ->
-      r:engine_record_repr {
-        l0_is_authentic r /\
-        EngineCore.cdi_functional_correctness cdi uds r
-      } ->
-      state_t
+  | G_UnInitialized, _
+  | _, G_UnInitialized -> False
 
-  | L1:
-      hndl:ctxt_hndl_t ->
-      r:l1_context_repr_t {
-        valid_hkdf_ikm_len dice_digest_len /\
-        L0Core.aliasKey_functional_correctness
-                    dice_hash_alg dice_digest_len r.cdi r.repr.fwid
-                    r.aliasKey_label_len r.repr.aliasKey_label 
-                    r.aliasKey_pub r.aliasKey_priv  /\ 
-        L0Core.deviceIDCSR_functional_correctness  
-                    dice_hash_alg dice_digest_len r.cdi
-                    r.deviceID_label_len r.repr.deviceID_label r.deviceIDCSR_ingredients 
-                    r.deviceIDCSR_len r.deviceIDCSR  /\      
-        L0Core.aliasKeyCRT_functional_correctness 
-                    dice_hash_alg dice_digest_len r.cdi r.repr.fwid
-                    r.deviceID_label_len r.repr.deviceID_label r.aliasKeyCRT_ingredients 
-                    r.aliasKeyCRT_len r.aliasKeyCRT r.aliasKey_pub
-      } ->
-      state_t
+  | G_SessionStart, G_Available (Engine_context_repr _)
+  | G_Available (Engine_context_repr _), G_Available (L0_context_repr _)
+  | G_Available (L0_context_repr _), G_Available (L1_context_repr _) -> True
 
-  | SessionClosed:
-      state_t
+  | G_SessionClosed _, _
+  | G_SessionError _, _ -> False
 
-let next (s0 s1:state_t) =
-    match s0, s1 with
-    | SessionStart _, EngineInitialized _ _ -> True
-    | EngineInitialized _ uds, L0 _ uds' cdi r -> uds==uds'
-    | L0 _ _ cdi _, L1 _ l1_ctxt -> cdi == l1_ctxt.cdi
-    (* destroy context preserving history *)
-    | EngineInitialized _ _, SessionStart (Some h)
-    | L0 _ _ _ _, SessionStart (Some h)
-    | L1 _ _, SessionStart (Some h) -> 
-      h == s0
-    | _ -> False
+  | _, G_SessionClosed s
+  | _, G_SessionError s -> s == s0
 
-let leads_to x y : prop = 
-    squash (FStar.ReflexiveTransitiveClosure.closure next x y)
+  | _, G_InUse s -> s == s0
 
-let rec well_formed_trace (l:list state_t) =
-    match l with
-    | [] -> True //empty trace
-    | [SessionStart None] -> True //singleton trace begins with SessionStart
-    | s1::s0::tl -> next s0 s1 /\ well_formed_trace (s0::tl)
-    | _ -> False
+  | G_InUse s, s1 -> next s s1
 
-type trace : Type u#1 = l:list state_t { well_formed_trace l }
+  | _ -> False
 
-let trace_extension (t0 t1:trace)
-  : prop
-  = Cons? t1 /\ t0 == List.Tot.tail t1
+let rec well_formed_trace (l:list g_session_state) =
+  match l with
+  | []
+  | [G_SessionStart] -> True
+  | s1::s0::tl -> next s0 s1 /\ well_formed_trace (s0::tl)
+  | _ -> False
 
-let trace_preorder
-  : FStar.Preorder.preorder trace
-  = FStar.ReflexiveTransitiveClosure.closure trace_extension
+type trace_elt : Type u#1 = l:list g_session_state { well_formed_trace l }
+
+let trace_extension (t0 t1:trace_elt) : prop =
+  Cons? t1 /\ t0 == List.Tot.tail t1
+
+let trace_preorder : FStar.Preorder.preorder trace_elt =
+  FStar.ReflexiveTransitiveClosure.closure trace_extension
 
 open FStar.PCM
 open FStar.Preorder
 open PulseCore.Preorder
 open PulseCore.FractionalPermission
 
-type pcm_carrier (#a:Type u#a) (p:preorder a) : Type u#a =
-  option (perm & bool) & hist p
+type trace = hist trace_preorder
 
-let pcm_composable #a (p:preorder a) : symrel (pcm_carrier p) =
+type pcm_t : Type u#1 = option perm & trace
+
+let pcm_composable : symrel pcm_t =
   fun x0 x1 -> 
   match x0, x1 with
   | (None, t0), (None, t1) -> t0 `extends` t1 \/ t1 `extends` t0
   | (Some _, t0), (None, t1) -> t0 `extends` t1
   | (None, t0), (Some _, t1) -> t1 `extends` t0
-  | (Some (p0, b0), t0), (Some (p1, b1), t1) ->
-    b0 == b1 /\
-    t0 == t1 /\
-    sum_perm p0 p1 `lesser_equal_perm` full_perm
+  | (Some p0, t0), (Some p1, t1) -> t0 == t1 /\ (p0 +. p1) <=. 1.0R
 
-let pcm_op #a (p:preorder a)
-  (x:pcm_carrier p)
-  (y:pcm_carrier p { pcm_composable p x y })
-  : pcm_carrier p =
-
+let pcm_op (x:pcm_t) (y:pcm_t { pcm_composable x y }) : pcm_t =
   match x, y with
-  | (None, t0), (None, t1) -> None, p_op p t0 t1
+  | (None, t0), (None, t1) -> None, p_op trace_preorder t0 t1
   | (Some _, _), (None, _) -> x
   | (None, _), (Some _, _) -> y
-  | (Some (p0, b0), t0), (Some (p1, _), t1) -> Some (sum_perm p0 p1, b0), t0
+  | (Some p0, t0), (Some p1, t1) -> Some (p0 +. p1), t0
 
-let pcm_one (#a:Type) (p:preorder a) : pcm_carrier p = None, []
+let pcm_one : pcm_t = None, []
 
-let pcm' (#a:Type) (p:preorder a) : pcm' (pcm_carrier p) = {
-  composable = pcm_composable p;
-  op = pcm_op p;
-  one = pcm_one p;
+let pcm' : pcm' pcm_t = {
+  composable = pcm_composable;
+  op = pcm_op;
+  one = pcm_one;
 }
 
-let lem_commutative (#a:Type) (p:preorder a) : lem_commutative (pcm' p) =
+let lem_commutative : lem_commutative pcm' =
   fun _ _ -> ()
 
-let lem_assoc_l (#a:Type) (p:preorder a) : lem_assoc_l (pcm' p) =
-  fun x y z ->
-  match x, y, z with
-  | (Some (_, _), _), (Some (_, _), _), (Some (_, _), _) -> ()
-  | _ -> ()
+let lem_assoc_l : lem_assoc_l pcm' =
+  fun _ _ _ -> ()
 
-let lem_assoc_r (#a:Type) (p:preorder a) : lem_assoc_r (pcm' p) =
-  fun x y z ->
-  match x, y, z with
-  | (Some (_, _), _), (Some (_, _), _), (Some (_, _), _) -> ()
-  | _ -> ()
+let lem_assoc_r : lem_assoc_r pcm' =
+  fun _ _ _ -> ()
 
-let rec extends_nil (#a:Type) (#p:preorder a) (l:hist p)
-  : Lemma (l `extends` []) =
-
+let rec extends_nil (l:trace) : Lemma (l `extends` []) =
   match l with
   | [] -> ()
-  | _::tl -> extends_nil #a #p tl
+  | _::tl -> extends_nil tl
 
-let lem_is_unit (#a:Type) (p:preorder a) : FStar.PCM.lem_is_unit (pcm' p) =
+let lem_is_unit : FStar.PCM.lem_is_unit pcm' =
   fun x ->
   match x with
   | Some _, t -> extends_nil t
-  | None, t -> p_op_nil p t
+  | None, t -> p_op_nil trace_preorder t
 
-let pcm (#a:Type) (p:preorder a) : pcm (pcm_carrier p) = {
-  p = pcm' p;
-  comm = lem_commutative p;
-  assoc = lem_assoc_l p;
-  assoc_r = lem_assoc_r p;
-  is_unit = lem_is_unit p;
+let pcm : pcm pcm_t = {
+  p = pcm';
+  comm = lem_commutative;
+  assoc = lem_assoc_l;
+  assoc_r = lem_assoc_r;
+  is_unit = lem_is_unit;
   refine = (fun _ -> True);
 }
 
-let mk_frame_preserving_upd (#a:Type) (p:preorder a)
-  (t0:hist p) (x:a { qhistory p (x::t0) })
-  (b0 b1:bool)
-  : frame_preserving_upd (pcm p) (Some (full_perm, b0), t0) (Some (full_perm, b1), x::t0) =
-  fun _ ->
-  assert (forall frame. pcm_composable p frame (Some (full_perm, b0), t0) ==> fst frame == None);
-  Some (full_perm, b1), x::t0
+let current_state (t:trace) : g_session_state =
+  match t with
+  | [] -> G_UnInitialized
+  | hd::_ ->
+    match hd with
+    | [] -> G_UnInitialized
+    | s::_ -> s
 
-let mk_frame_preserving_upd_b (#a:Type) (p:preorder a)
-  (t:hist p)
-  (b0 b1:bool)
-  : frame_preserving_upd (pcm p) (Some (full_perm, b0), t) (Some (full_perm, b1), t) =
-  fun _ ->
-  assert (forall frame. pcm_composable p frame (Some (full_perm, b0), t) ==> fst frame == None);
-  Some (full_perm, b1), t
+let valid_transition (t:trace) (s:g_session_state) : prop = next (current_state t) s
 
-let snapshot (#a:Type) (#p:preorder a) (x:pcm_carrier p) : pcm_carrier p =
-  None, snd x
+let next_trace (t:trace) (s:g_session_state { valid_transition t s }) : trace =
+  match t with
+  | [] -> [[s]]
+  | hd::tl ->
+    match hd with
+    | [] -> [s]::t
+    | l -> (s::l)::t
 
-let snapshot_idempotent (#a:Type) (#p:preorder a) (x:pcm_carrier p)
+let mk_frame_preserving_upd
+  (t:hist trace_preorder)
+  (s:g_session_state { valid_transition t s })
+  : frame_preserving_upd pcm (Some 1.0R, t) (Some 1.0R, next_trace t s) =
+  fun _ -> Some 1.0R, next_trace t s
+
+let snapshot (x:pcm_t) : pcm_t = None, snd x
+
+let snapshot_idempotent (x:pcm_t)
   : Lemma (snapshot x == snapshot (snapshot x)) = ()
 
-let snapshot_duplicable (#a:Type) (#p:preorder a) (x:pcm_carrier p)
+let snapshot_duplicable (x:pcm_t)
   : Lemma
       (requires True)
-      (ensures x `pcm_composable p` snapshot x) = ()
+      (ensures x `pcm_composable` snapshot x) = ()
 
-let full_perm_empty_history_compatible (#a:Type) (p:preorder a) (b:bool)
-  : Lemma (compatible (pcm p) (Some (full_perm, b), []) (Some (full_perm, b), [])) =
+let full_perm_empty_history_compatible ()
+  : Lemma (compatible pcm (Some 1.0R, []) (Some 1.0R, [])) =
   ()
 
 
